example/Fir.Check.fst
@@ -26,7 +26,7 @@ let bibo2_body (n: pos) (signal: reals): bools =
 
 let bibo2 n: reals -> bools =
   let e = Check.exp_of_stream1 (bibo2_body n) in
-  assert (Check.system_induct_k1 e) by (T.norm_full ());
+  assert (Check.system_induct_k1 e) by (T.norm_full ["Fir.Check"]);
   Check.stream_of_checked1 e
 
 let fir3 (input: reals): reals = fir [0.7R; 0.2R; 0.1R] input
@@ -36,5 +36,5 @@ let bibo3_body (n: pos) (signal: reals): bools =
 
 let bibo3 n: reals -> bools =
   let e = Check.exp_of_stream1 (bibo3_body n) in
-  assert (Check.system_induct_k 2 e) by (T.norm_full ());
+  assert (Check.system_induct_k 2 e) by (T.norm_full ["Fir.Check"]);
   Check.stream_of_checked1 e
