src/PipitRuntime.Prim.Bool.fst
@@ -1,0 +1,15 @@
+module PipitRuntime.Prim.Bool
+
+let p'b'not (x: bool): bool = not x
+
+let p'b'and (x y: bool): bool =
+  if x then y else false
+
+let p'b'or (x y: bool): bool =
+  if x then true else y
+
+let p'b'implies (x y: bool): bool =
+  if x then y else true
+
+let p'select (#a: Type) (cond: bool) (t f: a): a =
+  if cond then t else f
